Added proof draft

src/Core.v
@@ -100,7 +100,7 @@ Definition committed : Commit.id -> Prop :=
 Record wf := {
     wf_G : Wf G;
     cont_defined : forall e (NINIT : ~ is_init e) (IN : E e) (NRMW : ~ dom_rel rmw e),
-        is_some (cont X (CEvent e));
+    is_some (cont X (CEvent e));
     cont_init : forall tid (IN : threads_set tid), is_some (cont X (CInit tid));
     (* TODO: add property stating existence of continuation for some threads *)
 
@@ -137,9 +137,11 @@ Definition add_step_exec
            (X X' : t) : Prop :=
   let G' := G X' in
   let G := G X in
+  ⟪ WF_G' : Wf G' ⟫ /\
   ⟪ EDEF    :
     match e, e' with
     | InitEvent _, _ => False
+    | _, Some (InitEvent _) => False
     | ThreadEvent t n, Some (ThreadEvent t' n') =>
       t' = t /\ n' = 1 + n
     | _, _ => True
@@ -161,6 +163,8 @@ Definition add_step_exec
     ⟪ CO'     : co G ⊆ co G' ⟫ /\
     ⟪ RMW'   : rmw G' ≡ rmw G ∪ rmw_delta e e' ⟫.
 
+(* NOTE: merge this definition with add_step_exec? Or move parts of add_step_exec here? *)
+(* NOTE: should we add a requirement that `non_commit_ids` remain the same? *)
 Definition add_step_
            (e  : actid)
            (e' : option actid)
@@ -170,6 +174,60 @@ Definition add_step_
     add_step_exec lang k k' st st' e e' X X'.
 
 Definition add_step (X X' : t) : Prop := exists e e', add_step_ e e' X X'.
+
+Lemma add_step_same_uncommitted (X X' : t) (STEP : add_step X X') : non_commit_ids X' ≡₁ non_commit_ids X.
+Proof.
+Admitted.
+
+Lemma add_step_wf (X X' : t) (WF : wf X) (STEP : add_step X X') : wf X'.
+Proof.
+  unfold add_step, add_step_, add_step_exec in *.
+  desf; constructor; auto; intros.
+  { rewrite CONT'.
+    (* TODO turn into a lemma like set_subset_eq *)
+    apply set_subset_eq with (P := set_compl _) (a := e) in NRMW.
+    rewrite RMW', dom_union, set_compl_union in NRMW.
+    apply EVENTS in IN; unfolder in IN; desf.
+    { rewrite updo. apply WF; auto.
+      { apply set_subset_eq with (P := set_compl _) (a := e); auto.
+        now apply NRMW. }
+      injection as Heq.
+      apply EVENT with (x := e); simpl; unfolder; auto. }
+    { exfalso.
+      apply NRMW with (x := ThreadEvent thread index); auto.
+      unfold rmw_delta; unfolder; eauto. }
+    now rewrite upds. }
+  { rewrite CONT'.
+    rewrite updo by congruence.
+    apply WF. now apply THREADS. }
+  { (*
+    committed sets are the same.
+    therefore we probably should be able to prove that the
+    non_commit_ids set is the same
+    *)
+    admit. }
+  { admit. }
+  { admit. }
+  { rewrite CONT'.
+    (* TODO turn into a lemma like set_subset_eq *)
+    apply set_subset_eq with (P := set_compl _) (a := e) in NRMW.
+    rewrite RMW', dom_union, set_compl_union in NRMW.
+    apply EVENTS in IN; unfolder in IN; desf.
+    { rewrite updo. apply WF; auto.
+      { apply set_subset_eq with (P := set_compl _) (a := e); auto.
+        now apply NRMW. }
+      injection as Heq.
+      apply EVENT with (x := e); simpl; unfolder; auto. }
+    { simpl. now rewrite upds. }
+  }
+  { rewrite CONT'.
+    rewrite updo by congruence.
+    apply WF. now apply THREADS. }
+  { admit. }
+  { admit. }
+  { admit. }
+Qed.
+
 
 Record commit_step
            (cid : Commit.id)
